MiniML.v
@@ -1,0 +1,196 @@
+Require Import String.
+Require Import Names.
+Require Import PNames.
+Require Import Arith.
+Require Import Bool.
+Require Import Lambda.
+Require Import Arith_Lambda.
+Require Import Bool_Lambda.
+Require Import Polynomial.
+Require Import Containers.
+Require Import Functors.
+Require Import Mu.
+Require Import NatCase.
+
+Section MiniML.
+
+  Open Scope string_scope.
+
+  Definition D := AType :+: LType :+: BType.
+
+  Global Instance Container_D : Container D :=
+    PolynomialContainer D.
+
+  Global Instance SPF_D : SPF D.
+    eauto with typeclass_instances.
+  Defined.
+
+  Definition E (A : Set) := Arith :+: (Lambda D A) :+: Bool :+: (Fix_ D A) :+: (NatCase A).
+
+  Global Instance Container_E : forall (A : Set), Container (E A).
+    eauto with typeclass_instances.
+  Defined.
+
+  Definition letrec (A : Set) (t : DType D) (def : A -> Exp E A) (body : A -> Exp E A) :
+    (Exp E A) := app D E (lam _ _ t body) (mu _ _ t def).
+
+  Instance D_typeof T : FAlgebra TypeofName T (typeofR D) (E (typeofR D)).
+    eauto with typeclass_instances.
+  Defined.
+
+  Definition V := StuckValue :+: BotValue :+: NatValue :+: (ClosValue E) :+: (BoolValue).
+
+  Global Instance Container_V : Container V.
+    eauto with typeclass_instances.
+  Defined.
+
+  Instance V_eval : FAlgebra EvalName (Exp E nat) (evalR V) (E nat).
+    eauto 150 with typeclass_instances.
+  Defined.
+
+  (* Global Instance eq_DType_eq_D : *)
+  (*   PAlgebra eq_DType_eqName (sig (UP'_P (eq_DType_eq_P D))) D. *)
+  (* Proof. *)
+  (*   unfold D. *)
+  (*   eauto 20 with typeclass_instances. *)
+  (* Defined. *)
+
+  Definition Eqv (A B : Set) :=
+    (NP_Functor_eqv E Arith A B) ::+:: (NP_Functor_eqv E Bool A B) ::+::
+    (Lambda_eqv D E A B) ::+:: (Fix_eqv D E A B) ::+:: (NatCase_eqv E A B).
+
+  Definition WFV := (WFValue_Clos D E V Eqv (typeof _ _)) ::+::
+    (WFValue_Bot D V) ::+:: (WFValue_VI D V) ::+:: (WFValue_VB D V).
+
+  Global Instance Container_WFV : IContainer WFV.
+    eauto with typeclass_instances.
+  Defined.
+
+  Definition SV := (SubValue_refl V) ::+:: (SubValue_Bot V) ::+:: (SubValue_Clos E V).
+
+  Global Instance Container_SV : IContainer SV.
+    eauto with typeclass_instances.
+  Defined.
+
+  Global Instance SV_invertVI_SV :
+    iPAlgebra SV_invertVI_Name (SV_invertVI_P V) SV.
+    repeat apply iPAlgebra_Plus; eauto 150 with typeclass_instances.
+    constructor.
+    unfold iAlgebra.
+    unfold SV_invertVI_P.
+    intros i H n H0.
+    inversion H; subst.
+    elimtype False; apply (inject_discriminate _ _ _ H0).
+  Defined.
+
+  Global Instance SV_invertVI'_SV :
+    iPAlgebra SV_invertVI'_Name (SV_invertVI'_P V) SV.
+    repeat apply iPAlgebra_Plus; eauto 150 with typeclass_instances.
+    constructor.
+    unfold iAlgebra.
+    unfold SV_invertVI'_P.
+    intros i H n H0.
+    inversion H; subst.
+    elimtype False; apply (inject_discriminate _ _ _ H0).
+  Defined.
+
+  Global Instance SV_invertVB_SV :
+    iPAlgebra SV_invertVB_Name (SV_invertVB_P V) SV.
+    repeat apply iPAlgebra_Plus; eauto 150 with typeclass_instances.
+    constructor.
+    unfold iAlgebra.
+    unfold SV_invertVB_P.
+    intros i H n H0.
+    inversion H; subst.
+    elimtype False; apply (inject_discriminate _ _ _ H0).
+  Defined.
+
+  Global Instance SV_invertVB'_SV :
+    iPAlgebra SV_invertVB'_Name (SV_invertVB'_P V) SV.
+    repeat apply iPAlgebra_Plus; eauto 150 with typeclass_instances.
+    constructor.
+    unfold iAlgebra.
+    unfold SV_invertVB'_P.
+    intros i H n H0.
+    inversion H; subst.
+    elimtype False; apply (inject_discriminate _ _ _ H0).
+  Defined.
+
+  Global Instance EV_Alg :
+    FPAlgebra (eval_continuous_Exp_P V (E nat) SV) (inject (E nat) (E nat)).
+  Proof.
+    repeat apply FPAlgebra_Plus_cont_inject; eauto 200 with typeclass_instances.
+    - generalize (@Lambda_eval_continuous_Exp D _ _ _ E _ _ _ _).
+      eauto 200 with typeclass_instances.
+    - generalize (@Fix_eval_continuous_Exp D _ _ _ E _ _ _ _).
+      eauto 200 with typeclass_instances.
+    - generalize (@NatCase_eval_continuous_Exp E _ _ _ _).
+      eauto 200 with typeclass_instances.
+  Defined.
+
+  Lemma eval_continuous : forall m,
+    forall (e : Exp E nat) (gamma gamma' : Env _),
+      forall n (Sub_G_G' : Sub_Environment V SV gamma gamma'),
+        m <= n ->
+        SubValueC _ SV (beval _ _ m e gamma) (beval _ _ n e gamma').
+    eapply beval_continuous; eauto 250 with typeclass_instances.
+  Qed.
+
+  Eval compute in ("Continuity of Evaluation Proven for MiniML!").
+
+  (* Global Instance Bool_sound P_bind P pb typeof_rec eval_rec : *)
+  (*   PAlgebra eval_Soundness_alg_Name *)
+  (*   (sig (UP'_P2 (eval_alg_Soundness_P D V (E nat) WFV P_bind P *)
+  (*     (E (typeofR D)) (Fun_E (typeofR D)) pb typeof_rec *)
+  (*     eval_rec f_algebra f_algebra))) Bool. *)
+  (* Proof. *)
+  (*   eauto 250 with typeclass_instances. *)
+  (* Defined. *)
+
+  Instance Eval_Soundness_alg :
+    forall
+      eval_rec : Names.Exp (E nat) -> evalR V,
+      iPAlgebra soundness_XName
+                (soundness_X'_P D V E Eqv WFV
+                                (typeof D (E (typeofR D))) eval_rec
+                                f_algebra f_algebra)
+                (Eqv (typeofR D) nat).
+  Proof.
+    assert (WF_FAlgebra_eval_Lambda :
+              WF_FAlgebra EvalName (Names.Exp (E nat)) (evalR V)
+                (Lambda D nat) (E nat) (MAlgebra_eval_Lambda D E V) V_eval).
+    eauto 500 with typeclass_instances.
+    intros.
+    repeat apply iPAlgebra_Plus.
+    - apply Lift_soundness_X_alg.
+      + eauto with typeclass_instances.
+      + apply eqv_eval_Soundness; eauto 250 with typeclass_instances.
+    - apply Lift_soundness_X_alg.
+      + eauto with typeclass_instances.
+      + apply eqv_eval_Soundness; eauto 250 with typeclass_instances.
+    - eapply Lambda_eqv_eval_soundness_alg; eauto 250 with typeclass_instances.
+    - eapply Fix_Soundness; eauto 250 with typeclass_instances.
+    - apply Lift_soundness_X_alg.
+      + eauto with typeclass_instances.
+      + eapply NatCase_eval_Soundness; eauto 250 with typeclass_instances.
+  Qed.
+
+  Theorem soundness : forall n gamma gamma' gamma'' e' e'',
+    E_eqvC _ Eqv gamma gamma' e' e'' ->
+    forall (WF_gamma : forall n b, lookup gamma' n = Some b ->
+      exists T, lookup gamma b = Some T)
+    (WF_gamma2 : List.length gamma = List.length gamma')
+    (WF_gamma' : forall n b, lookup gamma' n = Some b -> b = n)
+    (WF_gamma'' : WF_Environment _ _ WFV gamma'' gamma) T,
+    typeof D (E _) e' = Some T -> WFValueC _ _ WFV (beval _ _ n e'' gamma'') T.
+  Proof.
+    eapply soundness_X; eauto 800 with typeclass_instances.
+    repeat apply iPAlgebra_Plus; eauto 800 with typeclass_instances.
+    apply (@WFV_Value_continuous_Clos D _ _ _ _ E _ _ _ V _ _ _ _ Eqv _ _ WFV _ _
+                                      (typeof D (E (typeofR D))));
+    eauto 800 with typeclass_instances.
+  Qed.
+
+  Eval compute in ("Type Soundness for MiniML Proven!").
+
+End MiniML.
